compiler/backend/passes/proofs/thunk_split_Forcing_LamProofScript.sml
@@ -1,0 +1,1513 @@
+
+
+open HolKernel Parse boolLib bossLib term_tactic pairTheory listTheory;
+open stringTheory optionTheory sumTheory pairTheory listTheory alistTheory
+     finite_mapTheory pred_setTheory rich_listTheory
+     dep_rewrite wellorderTheory arithmeticTheory;
+open mlmapTheory mlstringTheory var_setTheory thunk_cexpTheory;
+open pure_miscTheory thunkLangPropsTheory thunkLangTheory thunkLang_primitivesTheory
+     thunk_cexpTheory thunk_exp_ofTheory thunk_semanticsTheory thunk_NRC_Forcing_LambdasTheory var_setTheory
+     thunk_split_Forcing_LamTheory;
+
+val _ = new_theory "thunk_split_Forcing_LamProof";
+
+Theorem extract_names_list_soundness:
+  (∀l. (∀e. cexp_size e < list_size cexp_size l ⇒
+            cexp_wf e ⇒
+            set_of (extract_names e) = freevars (exp_of e) ∧ vars_ok (extract_names e)) ⇒
+       ∀s. vars_ok s ∧ EVERY cexp_wf l ⇒ set_of (extract_names_list s l) = set_of s
+                                                          ∪ (BIGUNION $ set (MAP (λe. freevars (exp_of e)) l)) ∧
+                       vars_ok (extract_names_list s l))
+Proof
+  Induct >> gs [extract_names_def, list_size_def] >>
+  simp [UNION_ASSOC]
+QED
+
+Theorem extract_names_rows_soundness:
+  (∀l. (∀e. cexp_size e < list_size (cexp_size o SND o SND) l ⇒
+            cexp_wf e ⇒
+            set_of (extract_names e) = freevars (exp_of e) ∧ vars_ok (extract_names e)) ⇒
+       ∀s. vars_ok s ∧ EVERY cexp_wf (MAP (SND o SND) l) ⇒
+           set_of (extract_names_rows s l)
+           = set_of s ∪ (BIGUNION $ set (MAP (λ(_, vs, e). freevars (exp_of e) DIFF set (MAP explode vs)) l)) ∧
+           vars_ok (extract_names_rows s l))
+Proof
+  Induct >> gs [extract_names_def, list_size_def] >>
+  PairCases >>
+  gs [extract_names_def, UNION_ASSOC]
+QED
+
+Theorem list_size_MAP:
+  ∀l f g. list_size f (MAP g l) = list_size (f o g) l
+Proof
+  Induct >> gs [list_size_def]
+QED
+
+Theorem in_freevars_Disj:
+  ∀l n x. x ∈ freevars (Disj n l) ⇒ x = n
+Proof
+  Induct >> gs [FORALL_PROD, Disj_def, freevars_def] >>
+  rw [] >> gs []
+QED
+
+Theorem freevars_lets_for:
+  ∀l v n x len. freevars (lets_for len v n (MAPi (λi v. (i, v)) l) x) DELETE n = freevars x DIFF (n INSERT set l)
+Proof
+  Induct using SNOC_INDUCT
+  \\ simp [lets_for_def, indexedListsTheory.MAPi_APPEND, SNOC_APPEND, lets_for_APPEND, freevars_def]
+  \\ simp [SET_EQ_SUBSET, SUBSET_DEF]
+  \\ rw [] \\ simp []
+QED
+
+Theorem freevars_rows_of:
+  ∀rows n eopt.
+    rows ≠ [] ⇒
+    freevars (rows_of n rows eopt) =
+    {n}
+    ∪ BIGUNION (set (MAP (λ(_, vs, e). freevars e DIFF set vs) rows))
+    ∪ (case eopt of NONE => {} | SOME (_, e) => freevars e)
+Proof
+  Induct >> simp [FORALL_PROD, rows_of_def, freevars_def] >>
+  rename1 ‘rows_of _ rows _’ >>
+  Cases_on ‘rows = []’
+  >- (simp [rows_of_def] >>
+      simp [SET_EQ_SUBSET, SUBSET_DEF] >> rw [] >>
+      rename1 ‘x = n ∨ _’ >> Cases_on ‘x = n’ >> simp []
+      >- (rename1 ‘lets_for (LENGTH l) m n (MAPi _ l) e’ >>
+          qspecl_then [‘l’, ‘m’, ‘n’, ‘e’, ‘LENGTH l’] assume_tac freevars_lets_for >>
+          gs [SET_EQ_SUBSET, SUBSET_DEF])
+      >- (CASE_TAC >> gs [freevars_def] >>
+          CASE_TAC >> gs [freevars_def] >>
+          dxrule_then assume_tac in_freevars_Disj >> gs [])
+      >- (rename1 ‘lets_for (LENGTH l) m n (MAPi _ l) e’ >>
+          qspecl_then [‘l’, ‘m’, ‘n’, ‘e’, ‘LENGTH l’] assume_tac freevars_lets_for >>
+          gs [SET_EQ_SUBSET, SUBSET_DEF])
+      >- (CASE_TAC >> gs [] >>
+          CASE_TAC >> gs [freevars_def])) >>
+  gs [] >>
+  last_x_assum kall_tac >>
+  rw [SET_EQ_SUBSET, SUBSET_DEF] >> gs [] >>
+  rename1 ‘x = n ∨ _’ >> Cases_on ‘x = n’ >> simp [] >>
+  rename1 ‘lets_for (LENGTH l) m n (MAPi _ l) e’ >>
+  qspecl_then [‘l’, ‘m’, ‘n’, ‘e’, ‘LENGTH l’] assume_tac freevars_lets_for >>
+  gs [SET_EQ_SUBSET, SUBSET_DEF]
+QED
+
+Theorem thunk_names_soundness:
+  cexp_wf e ⇒ set_of (thunk_names e) = freevars (exp_of e) ∧ vars_ok (thunk_names e)
+Proof
+  simp [thunk_names_def]
+  \\ completeInduct_on ‘cexp_size e’
+  \\ Cases \\ simp [extract_names_def, exp_of_def,freevars_def, cexp_wf_def]
+  >~[‘cexp_size (Prim c l)’]
+  >- (strip_tac >> strip_tac >>
+      qspec_then ‘l’ mp_tac extract_names_list_soundness >>
+      impl_tac
+      >- (gs [cexp_size_def] >>
+          gen_tac >> strip_tac >> strip_tac >>
+          last_x_assum irule >>
+          simp [GSYM size_eq]) >>
+      fs [SF ETA_ss] >>
+      simp [MAP_MAP_o, combinTheory.o_DEF])
+  >~[‘cexp_size (App e l)’]
+  >- (strip_tac >> qspec_then ‘l’ mp_tac extract_names_list_soundness >>
+      impl_tac
+      >- (gs [cexp_size_def] >>
+          gen_tac >> strip_tac >> strip_tac >>
+          last_x_assum irule >>
+          simp [GSYM size_eq]) >>
+      simp [SF ETA_ss] >>
+      gs [freevars_Apps, PULL_FORALL, cexp_size_def, MAP_MAP_o, combinTheory.o_DEF])
+  >~[‘cexp_size (Lam l e)’]
+  >- (strip_tac >>
+      last_x_assum $ qspec_then ‘cexp_size e’ assume_tac >>
+      gs [cexp_size_def, freevars_Lams])
+  >~[‘cexp_size (Let opt e1 e2)’]
+  >- (strip_tac >> gs [PULL_FORALL] >>
+      last_assum $ qspec_then ‘e1’ assume_tac >>
+      last_x_assum $ qspec_then ‘e2’ assume_tac >>
+      gs [cexp_size_def] >>
+      Cases_on ‘opt’ >> simp [extract_names_def, freevars_def, EXTENSION])
+  >~[‘cexp_size (Letrec l e)’]
+  >- (strip_tac >> strip_tac >>
+      qspec_then ‘MAP SND l’ mp_tac extract_names_list_soundness >>
+      impl_tac
+      >- (gs [cexp_size_def] >>
+          gen_tac >> strip_tac >> strip_tac >>
+          last_x_assum irule >>
+          simp [size_eq2]) >>
+      gs [PULL_FORALL] >>
+      last_x_assum $ qspec_then ‘e’ assume_tac >>
+      gs [cexp_size_def, EVERY_MAP, EVERY_MEM] >>
+      disch_then $ drule_then assume_tac >> gs [FORALL_PROD, SF DNF_ss] >>
+      first_x_assum $ drule_then assume_tac >>
+      first_x_assum $ drule_then assume_tac >>
+      simp [MAP_MAP_o, combinTheory.o_DEF, LAMBDA_PROD])
+  >~[‘cexp_size (Case n rows eopt)’]
+  >- (strip_tac >> strip_tac >>
+      qspec_then ‘rows’ mp_tac extract_names_rows_soundness >>
+      impl_tac
+      >- (gs [cexp_size_def] >>
+          gen_tac >> strip_tac >> strip_tac >>
+          last_x_assum irule >>
+          simp [size_eq_case, list_size_MAP]) >>
+      disch_then $ qspec_then ‘case eopt of NONE => empty_vars | SOME (a,e) => extract_names e’ mp_tac >>
+      impl_tac
+      >- (conj_tac
+          >- (CASE_TAC >> simp [] >> CASE_TAC >> gs [cexp_size_def]) >>
+          gs [EVERY_MEM, MEM_MAP, PULL_EXISTS, FORALL_PROD] >>
+          rw [] >> last_x_assum $ drule_then assume_tac >> gs []) >>
+      simp [freevars_rows_of] >>
+      disch_then kall_tac >>
+      rw [SET_EQ_SUBSET, SUBSET_DEF] >> gs []
+      >- (Cases_on ‘eopt’ >> gs [] >>
+          pairarg_tac >> gs [PULL_FORALL] >>
+          rename1 ‘extract_names e’ >>
+          last_x_assum $ qspec_then ‘e’ assume_tac >> gs [cexp_size_def])
+      >- (disj1_tac >> disj2_tac >>
+          first_x_assum $ irule_at Any >>
+          gs [MEM_MAP] >>
+          first_x_assum $ irule_at Any >>
+          pairarg_tac >> gs [])
+      >- (disj2_tac >> disj2_tac >>
+          first_x_assum $ irule_at Any >>
+          gs [MEM_MAP] >>
+          first_x_assum $ irule_at Any >>
+          pairarg_tac >> gs [] >>
+          pairarg_tac >> gs [])
+      >- (CASE_TAC >> gs [] >>
+          CASE_TAC >> gs [PULL_FORALL] >>
+          rename1 ‘extract_names e’ >>
+          last_x_assum $ qspec_then ‘e’ assume_tac >> gs [cexp_size_def]))
+  >~[‘cexp_size (Delay e)’]
+  >- (strip_tac >>
+      last_x_assum $ qspec_then ‘cexp_size e’ assume_tac >>
+      gs [cexp_size_def])
+  >~[‘cexp_size (Box e)’]
+  >- (strip_tac >>
+      last_x_assum $ qspec_then ‘cexp_size e’ assume_tac >>
+      gs [cexp_size_def])
+  >~[‘cexp_size (Force e)’]
+  >- (strip_tac >>
+      last_x_assum $ qspec_then ‘cexp_size e’ assume_tac >>
+      gs [cexp_size_def])
+QED
+
+Theorem boundvars_to_lets_force:
+  ∀l e v. v ∈ boundvars e ⇒ v ∈ boundvars (lets_force l e)
+Proof
+  Induct >> gs [lets_force_def, FORALL_PROD] >>
+  rw [] >> last_x_assum irule >>
+  simp [boundvars_def]
+QED
+
+Theorem freevars_to_lets_force:
+  ∀l e v. v ∈ freevars e ⇒ v ∈ freevars (lets_force l e) ∨ v ∈ boundvars (lets_force l e)
+Proof
+  Induct >> gs [lets_force_def, FORALL_PROD] >>
+  rw [] >>
+  rename1 ‘Let (SOME p1) (Force (Var p2)) e’ >>
+  rename1 ‘v ∈ _’ >>
+  Cases_on ‘v ∈ freevars (Let (SOME p1) (Force (Var p2)) e)’ >> gs [] >>
+  disj2_tac >>
+  irule boundvars_to_lets_force >>
+  gs [boundvars_def, freevars_def]
+QED
+
+Theorem in_freevars_lets_force:
+  ∀l e v. v ∈ freevars (lets_force l e) ⇒ v ∈ freevars e ∨ MEM v (MAP SND l)
+Proof
+  Induct >> gs [lets_force_def, FORALL_PROD] >>
+  rw [] >>
+  last_x_assum $ dxrule_then assume_tac >>
+  gs [freevars_def]
+QED
+
+Theorem FEQUAL:
+  ∀a b c. b = c ⇒ a b = a c
+Proof
+  simp []
+QED
+
+Theorem FEQUAL2:
+  ∀a b c. b = c ⇒ b a = c a
+Proof
+  simp []
+QED
+
+Theorem IMP_MEM_FILTER_merge_inside:
+  ∀l1 bL1 l2 bL2 v.
+    MEM v l2 ∧
+    LENGTH l1 = LENGTH bL1 ∧
+    LENGTH l2 = LENGTH (FILTER FST (ZIP (bL1, l1)))
+    ⇒ MEM v (MAP SND (FILTER FST (ZIP (bL1, merge_inside l1 bL1 l2))))
+Proof
+  Induct >> simp [merge_inside_def] >>
+  gen_tac >> Cases >> simp [] >>
+  IF_CASES_TAC >> gs []
+  >- (Cases >> simp [merge_inside_def, PULL_EXISTS] >>
+      rw [] >>
+      disj2_tac >> last_x_assum $ drule_then irule >>
+      gs []) >>
+  simp [merge_inside_def, PULL_EXISTS]
+QED
+
+Theorem EQ_LENGTH_FILTER_ZIP:
+  ∀bL l1 l2.
+    LENGTH l1 = LENGTH l2 ∧ LENGTH bL = LENGTH l1
+    ⇒ LENGTH (FILTER FST (ZIP (bL, l1))) = LENGTH (FILTER FST (ZIP (bL, l2)))
+Proof
+  Induct >> simp [] >>
+  Cases >> simp [] >>
+  Cases >> simp [] >>
+  Cases >> simp []
+QED
+
+Theorem find_forcing_soundness:
+  ∀l e l1 l2 bL e2 s b1 b2 s2.
+    find_forcing l e = (l1, l2, bL, e2, s, b1, b2, s2) ∧ cexp_wf e ⇒
+    ∃l3 bL2.
+      cexp_wf e2 ∧
+      l1 = MAP SND (FILTER FST (ZIP (bL2, l))) ∧
+      LENGTH l = LENGTH bL ∧
+      (∀v. v ∈ freevars (exp_of e2) ∪ boundvars (exp_of e2) ⇒ v ∈ freevars (exp_of e) ∪ boundvars (exp_of e)) ∧
+      (∀v. MEM v l3 ⇒ explode v ∈ boundvars (exp_of e)) ∧
+      LIST_REL (λb2 b. b2 ⇒ b) bL2 bL ∧
+      LIST_REL (λ(b, b2) v. b ⇒ (b2 ⇔ v ∈ freevars (exp_of e2))) (ZIP (bL, bL2)) (MAP explode l) ∧
+      LENGTH l3 = LENGTH (FILTER FST (ZIP (bL, l))) ∧
+      vars_ok s2 ∧ set_of s2 = set (MAP explode l3) ∪ set (MAP explode l) ∧
+      (b1 ⇔ MEM T bL) ∧
+      (b2 ⇒ ALL_DISTINCT (l ++ l3)) ∧
+      (exp_of e) = lets_force (REVERSE (ZIP (MAP explode $ MAP SND (FILTER FST (ZIP (bL, l2))),
+                                             MAP explode $ MAP SND (FILTER FST (ZIP (bL, l))))))
+                               (exp_of e2) ∧
+      set_of s = freevars (exp_of e2) ∧ vars_ok s ∧
+      l2 = merge_inside l bL l3
+Proof
+  Induct
+  >- (Cases >> gs [find_forcing_def, lets_force_def, thunk_names_soundness, merge_inside_def, cexp_wf_def]) >>
+  gen_tac >> Cases >> rpt gen_tac >> strip_tac >>
+  gvs [find_forcing_def, lets_force_def, thunk_names_soundness, merge_inside_def,
+      thunk_Forcing_LambdasTheory.FILTER_FST_ZIP_K_F, merge_inside_K_F, cexp_wf_def, PULL_EXISTS]
+  >>~-([‘LIST_REL _ _ (MAP (K F) l)’], qexists_tac ‘MAP (K F) l’ >>
+               gs [thunk_Forcing_LambdasTheory.FILTER_FST_ZIP_K_F, LIST_REL_EL_EQN, EL_ZIP, EL_MAP, MEM_MAP]) >>
+  rename1 ‘find_forcing (h::l) (Let opt x y)’ >>
+  Cases_on ‘x’ >>
+  gvs [find_forcing_def, lets_force_def, thunk_names_soundness, merge_inside_def,
+      thunk_Forcing_LambdasTheory.FILTER_FST_ZIP_K_F, merge_inside_K_F, cexp_wf_def, PULL_EXISTS]
+  >>~-([‘LIST_REL _ _ (MAP (K F) l)’], qexists_tac ‘MAP (K F) l’ >>
+               gs [thunk_Forcing_LambdasTheory.FILTER_FST_ZIP_K_F, LIST_REL_EL_EQN, EL_ZIP, EL_MAP, MEM_MAP]) >>
+  Cases_on ‘opt’ >>
+  gvs [find_forcing_def, lets_force_def, thunk_names_soundness, merge_inside_def,
+      thunk_Forcing_LambdasTheory.FILTER_FST_ZIP_K_F, merge_inside_K_F, cexp_wf_def, PULL_EXISTS]
+  >>~-([‘LIST_REL _ _ (MAP (K F) l)’], qexists_tac ‘MAP (K F) l’ >>
+               gs [thunk_Forcing_LambdasTheory.FILTER_FST_ZIP_K_F, LIST_REL_EL_EQN, EL_ZIP, EL_MAP, MEM_MAP]) >>
+  rename1 ‘find_forcing (h::l) (Let (SOME h2) (Force e) y)’ >>
+  Cases_on ‘e’ >>
+  gvs [find_forcing_def, lets_force_def, thunk_names_soundness, merge_inside_def,
+      thunk_Forcing_LambdasTheory.FILTER_FST_ZIP_K_F, merge_inside_K_F, cexp_wf_def, PULL_EXISTS]
+  >>~-([‘LIST_REL _ _ (MAP (K F) l)’], qexists_tac ‘MAP (K F) l’ >>
+               gs [thunk_Forcing_LambdasTheory.FILTER_FST_ZIP_K_F, LIST_REL_EL_EQN, EL_ZIP, EL_MAP, MEM_MAP]) >>
+  qpat_x_assum ‘_ _ = (_, _, _, _, _, _, _, _)’ mp_tac >>
+  IF_CASES_TAC
+  >- (pairarg_tac >> rw [] >>
+      last_x_assum $ dxrule_then assume_tac >>
+      gs [lets_force_APPEND, lets_force_def, PULL_EXISTS, merge_inside_def] >>
+      Q.REFINE_EXISTS_TAC ‘_::_’ >> gs [contains_var_in_set_of, merge_inside_def] >>
+      irule_at (Pos last) EQ_REFL >>
+      irule_at (Pos hd) EQ_REFL
+      >- (simp [freevars_def, boundvars_def] >>
+          rw []
+          >- (rename1 ‘freevars (lets_force big_list _)’ >>
+              dxrule_then (qspec_then ‘big_list’ assume_tac) freevars_to_lets_force >>
+              gs [])
+          >- (dxrule_then assume_tac boundvars_to_lets_force >> gs [])
+          >- (‘∀v : string s1 s2. v ∈ s2 ∧ s1 = s2 ⇒ v ∈ s1’ by simp [] >>
+              disj1_tac >> pop_assum irule >>
+              irule_at (Pos hd) FEQUAL >>
+              irule_at (Pos hd) FEQUAL2 >> irule_at (Pos hd) FEQUAL >>
+              irule_at Any REVERSE_ZIP >>
+              conj_asm1_tac
+              >- (simp [] >>
+                  irule EQ_LENGTH_FILTER_ZIP >>
+                  simp [LENGTH_merge_inside]) >>
+              simp [boundvars_lets_force] >>
+              disj2_tac >>
+              irule $ iffRL MEM_MAP >> irule_at Any EQ_REFL >>
+              irule IMP_MEM_FILTER_merge_inside >>
+              simp [])
+          >- simp [set_of_insert_var, vars_ok_insert_var, SET_EQ_SUBSET, SUBSET_DEF]
+          >- gs [MEM_MAP]
+          >- gs [MEM_MAP]
+          >- gs [ALL_DISTINCT_APPEND, MEM_MAP])
+      >- (simp [freevars_def, boundvars_def] >>
+          rw []
+          >- (rename1 ‘freevars (lets_force big_list _)’ >>
+              dxrule_then (qspec_then ‘big_list’ assume_tac) freevars_to_lets_force >>
+              gs [])
+          >- (dxrule_then assume_tac boundvars_to_lets_force >> gs [])
+          >- (‘∀v : string s1 s2. v ∈ s2 ∧ s1 = s2 ⇒ v ∈ s1’ by simp [] >>
+              disj1_tac >> pop_assum irule >>
+              irule_at (Pos hd) FEQUAL >>
+              irule_at (Pos hd) FEQUAL2 >> irule_at (Pos hd) FEQUAL >>
+              irule_at Any REVERSE_ZIP >>
+              conj_asm1_tac
+              >- (simp [] >>
+                  irule EQ_LENGTH_FILTER_ZIP >>
+                  simp [LENGTH_merge_inside]) >>
+              simp [boundvars_lets_force] >>
+              disj2_tac >>
+              irule $ iffRL MEM_MAP >> irule_at Any EQ_REFL >>
+              irule IMP_MEM_FILTER_merge_inside >>
+              simp [])
+          >- simp [set_of_insert_var, vars_ok_insert_var, SET_EQ_SUBSET, SUBSET_DEF]
+          >- gs [MEM_MAP]
+          >- gs [MEM_MAP]
+          >- gs [ALL_DISTINCT_APPEND, MEM_MAP]))
+  >- (pairarg_tac >> rw [] >> simp [cexp_wf_def, PULL_EXISTS] >>
+      last_x_assum $ dxrule_then assume_tac >> gs [merge_inside_def, cexp_wf_def] >>
+      irule_at (Pos last) EQ_REFL >> simp [] >>
+      irule_at (Pos hd) EQ_REFL >> simp [] >> rw []
+      >- (rename1 ‘freevars (lets_force big_list _)’ >>
+          dxrule_then (qspec_then ‘big_list’ assume_tac) freevars_to_lets_force >>
+          gs [])
+      >- (dxrule_then assume_tac boundvars_to_lets_force >> gs [])
+      >- simp [SET_EQ_SUBSET, SUBSET_DEF]
+      >- gs [contains_var_in_set_of, MEM_MAP]
+      >- gs [contains_var_in_set_of, MEM_MAP])
+QED
+
+Theorem exp_rel_Lams:
+  ∀l s x y. exp_rel s (Lams l x) (Lams l y) ⇔ exp_rel s x y
+Proof
+  Induct >> gs [exp_rel_def]
+QED
+
+Theorem my_function_Let_NONE:
+  ∀x y s. my_function s (Let NONE x y) =
+          let (s, x) = my_function s x in
+            let (s, y) = my_function s y in
+              (s, Let NONE x y)
+Proof
+  Cases >> simp [Once my_function_def]
+QED
+
+Definition dest_Lam_def:
+  dest_Lam (thunk_cexp$Lam l e) = SOME e ∧
+  dest_Lam e = NONE
+End
+
+Theorem my_function_test1:
+  SND (my_function (insert_vars empty_vars [«f»; «x»; «x2»])
+       (Let (SOME «f») (Lam [«x»] (Var «x»)) (Var «f»)))
+  = (Let (SOME «f») (Lam [«x»] (Var «x»)) (Var «f»))
+Proof
+  EVAL_TAC
+QED
+
+Theorem find_forcing_test:
+  find_forcing (REV [«x»] [])
+       (Let (SOME «y») (Force (Var «x»)) (Var «y»))
+  = ([],[«y»],[T],Var «y»,(Map compare (Bin 1 «y» () Tip Tip),1),T,T,
+     Map compare (Bin 2 «x» () Tip (Bin 1 «y» () Tip Tip)),1)
+Proof
+  EVAL_TAC
+QED
+
+(*Theorem my_function_test:
+  SND (my_function (insert_vars empty_vars [«f»; «x»; «y»])
+       (Let (SOME «f») (Lam [«x»] (Let (SOME «y») (Force (Var «x»)) (Var «y»))) (Var «f»)))
+  = Let (SOME «f») (Lam [«x»] (Let (SOME «y») (Force (Var «x»)) (Var «y»))) (Var «f»)
+Proof
+  simp [my_function_def, find_forcing_test] >>
+  simp [check_hypothesis_def] >>
+  simp [REV_REVERSE_LEM, contains_var_def, insert_vars_def, insert_var_def, lookup_def, empty_vars_def] >>
+  simp [empty_def, insert_def, balanced_mapTheory.lookup_def, balanced_mapTheory.empty_def,
+        balanced_mapTheory.insert_def, compare_def] >>
+  simp [compare_aux_def]
+   EVAL_TAC
+QED*)
+
+Theorem my_function_Let_SOME_dLam_is_NONE:
+  ∀x y v s. dest_Lam x = NONE ⇒
+          my_function s (Let (SOME v) x y) =
+          let (s, x) = my_function s x in
+            let (s, y) = my_function s y in
+              (s, Let (SOME v) x y)
+Proof
+  Cases >> simp [Once my_function_def, dest_Lam_def]
+QED
+
+Theorem REV_NOT_EMPTY:
+  ∀l1 l2. REV l1 l2 = [] ⇒ l1 = [] ∧ l2 = []
+Proof
+  Induct >> gs [REV_DEF] >>
+  rw [] >> strip_tac >>
+  last_x_assum $ dxrule_then assume_tac >> gs []
+QED
+
+Theorem REV_merge_inside:
+  ∀l bL l3.
+    merge_inside l bL l3 = [] ∧ LENGTH l3 = LENGTH (FILTER FST (ZIP (bL, l))) ∧ LENGTH l = LENGTH bL ⇒
+    l = []
+Proof
+  Induct >> simp [] >>
+  gen_tac >> Cases >> simp [] >>
+  IF_CASES_TAC >> simp [merge_inside_def] >>
+  Cases >> simp [merge_inside_def]
+QED
+
+Theorem exp_rel_Let_Lams_combine_bis:
+  ∀set v1 v2 vL vL1 vL2 vL3 vL4 bL bL2 x1 x2 y1 y2 expr1 expr2.
+    LENGTH vL = LENGTH bL ∧ MEM T bL ∧
+    vL1 = MAP SND (FILTER FST (ZIP (bL, vL))) ∧
+    LENGTH vL2 = LENGTH vL1 ∧
+    vL3 = MAP SND (FILTER FST (ZIP (bL2, vL))) ∧
+    LIST_REL (λ(b, b2) v. b ⇒ (b2 ⇔ v ∈ freevars x1)) (ZIP (bL, bL2)) vL ∧
+    LIST_REL (λb2 b. b2 ⇒ b) bL2 bL ∧
+    v2 ∉ set ∧
+    v2 ∉ freevars y1 ∧ v2 ∉ boundvars y2 ∧
+    v2 ∉ boundvars x1 ∧ v2 ∉ boundvars y1 ∧
+    ALL_DISTINCT (v1::v2::vL ++ vL2) ∧
+    vL4 = merge_inside vL bL vL2 ∧
+    exp_rel (set ∪ {v2}) x1 x2 ∧ exp_rel (set ∪ {v2}) y1 y2 ∧
+    expr1 = (Let (SOME v1)
+             (Lams vL (lets_force (ZIP (vL2, vL1)) x1)) y1) ∧
+    expr2 = (Let (SOME v2)
+             (Lams (vL3 ++ vL4) x2)
+             (Let (SOME v1)
+              (Lams vL (Apps (Var v2) (MAP Var vL3 ++
+                                       MAP2 (λb e. if b then Force e else e)
+                                            bL (MAP Var vL)))) y2)) ⇒
+    exp_rel set expr1 expr2
+Proof
+  rw [] >> irule exp_rel_Let_Lams_combine >> simp [] >>
+  rpt $ first_x_assum $ irule_at Any >>
+  simp []
+QED
+
+Theorem exp_rel_lets_force_left:
+  ∀l c e set. exp_rel set c (lets_force l e) ⇒ ∃e1. c = lets_force l e1 ∧ exp_rel set e1 e
+Proof
+  Induct >> gs [lets_force_def, FORALL_PROD] >>
+  rw [] >> last_x_assum $ dxrule_then assume_tac >>
+  gs [] >>
+  rename1 ‘exp_rel _ e1 _’ >>
+  Cases_on ‘e1’ >> gs [exp_rel_def]
+  >- (rename1 ‘exp_rel _ e1 (Force _)’ >>
+      Cases_on ‘e1’ >> gs [exp_rel_def] >>
+      rename1 ‘exp_rel _ e1 (Var _)’ >>
+      Cases_on ‘e1’ >> gs [exp_rel_def] >>
+      metis_tac []) >>
+  rename1 ‘Force _ = Lams (l1 ++ merge_inside vL bL vL2) _’ >>
+  Cases_on ‘l1’ >> gs [] >>
+  Cases_on ‘vL’ >> Cases_on ‘bL’ >> gs []
+  >- (Cases_on ‘vL2’ >> gs [merge_inside_def]) >>
+  rename1 ‘merge_inside _ (h2::_) vL2’ >>
+  Cases_on ‘h2’ >> gs [merge_inside_def] >>
+  Cases_on ‘vL2’ >> gs [merge_inside_def]
+QED
+
+Theorem MAP_FILTER_ZIP:
+  ∀bL vL f. LENGTH bL = LENGTH vL ⇒
+            MAP f (MAP SND (FILTER FST (ZIP (bL, vL)))) = MAP SND (FILTER FST (ZIP (bL, MAP f vL)))
+Proof
+  Induct >> gs [] >>
+  Cases >> Cases >> gs []
+QED
+
+Theorem merge_inside_APPEND:
+  ∀vL bL l2 vL' bL' l2'.
+    LENGTH l2 = LENGTH (FILTER FST (ZIP (bL, vL))) ∧ LENGTH bL = LENGTH vL
+    ⇒ merge_inside (vL ++ vL') (bL ++ bL') (l2 ++ l2')
+      = merge_inside vL bL l2 ++ merge_inside vL' bL' l2'
+Proof
+  Induct >> gs [merge_inside_def] >>
+  gen_tac >> Cases >> gs [] >>
+  IF_CASES_TAC >> gs [merge_inside_def] >>
+  Cases >> gs [merge_inside_def]
+QED
+
+Theorem REVERSE_merge_inside:
+  ∀vL bL l2. LENGTH l2 = LENGTH (FILTER FST (ZIP (bL, vL))) ∧ LENGTH bL = LENGTH vL ⇒
+             REVERSE (merge_inside vL bL l2) = merge_inside (REVERSE vL) (REVERSE bL) (REVERSE l2)
+Proof
+  Induct >> gs [merge_inside_def] >>
+  gen_tac >> Cases >> gs [] >>
+  IF_CASES_TAC >> gs [merge_inside_def]
+  >- (Cases >> rw [merge_inside_def] >>
+      irule EQ_TRANS >>
+      irule_at (Pos last) $ GSYM merge_inside_APPEND >>
+      gs [merge_inside_def, GSYM REVERSE_ZIP, FILTER_REVERSE]) >>
+  rw [merge_inside_def] >>
+  irule EQ_TRANS >>
+  irule_at (Pos last) EQ_TRANS >>
+  irule_at (Pos hd) $ GSYM merge_inside_APPEND >>
+  irule_at (Pos last) FEQUAL >>
+  rename1 ‘[h] = merge_inside _ _ _’ >>
+  qexists_tac ‘[h]’ >> qexists_tac ‘[]’ >> qexists_tac ‘[F]’ >>
+  gs [merge_inside_def, GSYM REVERSE_ZIP, FILTER_REVERSE]
+QED
+
+Theorem MAP_merge_inside:
+  ∀bL vL l2 f. LENGTH l2 = LENGTH (FILTER FST (ZIP (bL, vL))) ∧ LENGTH bL = LENGTH vL ⇒
+               MAP f (merge_inside vL bL l2) = merge_inside (MAP f vL) bL (MAP f l2)
+Proof
+  Induct >> gs [merge_inside_def] >>
+  Cases >> Cases >> gs [merge_inside_def] >>
+  Cases >> gs [merge_inside_def]
+QED
+
+Theorem check_hypothesis_soundness:
+  ∀b v s l1 l2. check_hypothesis b v s ⇒ b ∧ (vars_ok s ⇒ explode v ∉ set_of s)
+Proof
+  simp [check_hypothesis_def] >>
+  rw [] >> gs [contains_var_in_set_of]
+QED
+
+Theorem MEM_MAP_ZIP:
+  ∀l1 l2 x. MEM x (MAP SND (ZIP (l1, l2))) ∧ LENGTH l1 = LENGTH l2 ⇒ MEM x l2
+Proof
+  rw [] >> gs [MAP_ZIP]
+QED
+
+Theorem my_function_list_lemma:
+  ∀l s l2 s2. my_function_list s l = (s2, l2) ∧
+              (∀e. cexp_size e < list_size cexp_size l ⇒
+                   ∀s. vars_ok s ∧ freevars (exp_of e) ⊆ set_of s ∧ cexp_wf e ∧ boundvars (exp_of e) ⊆ set_of s ⇒
+                       ∀s2 e2. (s2, e2) = my_function s e ⇒
+                               cexp_wf e2 ∧
+                               vars_ok s2 ∧ set_of s ⊆ set_of s2 ∧ boundvars (exp_of e2) ⊆ set_of s2 ∧
+                               freevars (exp_of e2) ⊆ set_of s2 ∧
+                               (∀s3. DISJOINT s3 (boundvars (exp_of e2) ∪ freevars (exp_of e2))
+                                     ⇒ exp_rel s3 (exp_of e) (exp_of e2))) ⇒
+              vars_ok s ∧
+              EVERY (λe. freevars (exp_of (e)) ⊆ set_of s ∧ cexp_wf e ∧ boundvars (exp_of e) ⊆ set_of s) l
+              ⇒ vars_ok s2 ∧ set_of s ⊆ set_of s2 ∧
+                EVERY (λe. freevars (exp_of (e)) ⊆ set_of s2 ∧ cexp_wf e ∧ boundvars (exp_of e) ⊆ set_of s2) l2 ∧
+                (∀s3. EVERY (λe2. DISJOINT s3 (boundvars (exp_of e2) ∪ freevars (exp_of e2))) l2
+                      ⇒ LIST_REL (λe e2. exp_rel s3 (exp_of e) (exp_of e2)) l l2)
+Proof
+  Induct >> simp [my_function_def, PULL_EXISTS] >>
+  rpt $ gen_tac >>
+  pairarg_tac >>
+  rename [‘my_function_list _ l’, ‘my_function s h = (s', hd')’] >>
+  asm_rewrite_tac [PAIRED_BETA_CONV $
+                    Term ‘(λ(s',hd'). (λ(s'',tl'). (s'',hd'::tl')) (my_function_list s' l)) (s',hd')’] >>
+  pairarg_tac >>
+  last_x_assum $ drule_then assume_tac >>
+  rename1 ‘my_function_list s' l = (s'', tl')’ >>
+  asm_rewrite_tac [PAIRED_BETA_CONV $ Term ‘(λ(s'',tl'). (s'',hd'::tl')) (s'', tl')’] >>
+  strip_tac >> strip_tac >>
+  first_assum $ qspec_then ‘h’ mp_tac >>
+  impl_tac >- simp [list_size_def] >>
+  disch_then $ qspec_then ‘s’ mp_tac >>
+  impl_tac >- simp [] >>
+  disch_then $ qspecl_then [‘s'’, ‘hd'’] mp_tac >>
+  impl_tac >- simp [] >> strip_tac >>
+  qpat_x_assum ‘_ ⇒ _’ mp_tac >> impl_tac
+  >- (reverse conj_tac
+      >- (gs [EVERY_CONJ, EVERY_MEM] >>
+          rpt $ strip_tac >> rpt $ first_x_assum $ drule_then assume_tac >>
+          irule SUBSET_TRANS >>
+          first_x_assum $ irule_at $ Pos hd >> simp []) >>
+      gen_tac >> rename1 ‘cexp_size e < list_size _ _’ >>
+      first_x_assum $ qspec_then ‘e’ assume_tac >>
+      strip_tac >> qpat_x_assum ‘_ ⇒ _’ mp_tac >> impl_tac
+      >- simp [list_size_def] >>
+      strip_tac >> gen_tac >> strip_tac >> first_x_assum drule >>
+      rename1 ‘my_function s3 e’ >> Cases_on ‘my_function s3 e’ >> simp []) >>
+  strip_tac >> gs [] >>
+  conj_tac
+  >- (irule SUBSET_TRANS >> first_x_assum $ irule_at $ Pos hd >> simp []) >>
+  qpat_x_assum ‘_::_ = _’ assume_tac >>
+  dxrule_then assume_tac EQ_SYM >>
+  simp [] >> gs [EVERY_CONJ, EVERY_MEM] >>
+  conj_tac >> irule SUBSET_TRANS >> metis_tac []
+QED
+
+Theorem my_function_bind_lemma:
+  ∀l s l2 s2. my_function_bind s l = (s2, l2) ∧
+              (∀e. cexp_size e < list_size cexp_size (MAP SND l) ⇒
+                   ∀s. vars_ok s ∧ freevars (exp_of e) ⊆ set_of s ∧ cexp_wf e ∧ boundvars (exp_of e) ⊆ set_of s ⇒
+                       ∀s2 e2. (s2, e2) = my_function s e ⇒
+                               cexp_wf e2 ∧
+                               vars_ok s2 ∧ set_of s ⊆ set_of s2 ∧ boundvars (exp_of e2) ⊆ set_of s2 ∧
+                               freevars (exp_of e2) ⊆ set_of s2 ∧
+                               (∀s3. DISJOINT s3 (boundvars (exp_of e2) ∪ freevars (exp_of e2))
+                                     ⇒ exp_rel s3 (exp_of e) (exp_of e2))) ⇒
+           vars_ok s ∧
+           EVERY (λ(v, e). freevars (exp_of (e)) ⊆ set_of s ∧ cexp_wf e ∧ boundvars (exp_of e) ⊆ set_of s) l
+           ⇒ vars_ok s2 ∧ set_of s ⊆ set_of s2 ∧ MAP FST l = MAP FST l2 ∧
+             EVERY (λ(v, e). freevars (exp_of (e)) ⊆ set_of s2 ∧ cexp_wf e ∧ boundvars (exp_of e) ⊆ set_of s2) l2 ∧
+             (∀s3. EVERY (λ(v, e2). DISJOINT s3 (boundvars (exp_of e2) ∪ freevars (exp_of e2))) l2
+                   ⇒ LIST_REL (λ(v, e) (v2, e2). exp_rel s3 (exp_of e) (exp_of e2)) l l2) ∧
+             (EVERY (λ(_,x). cexp_ok_bind x ∧ cexp_wf x) l ⇒ EVERY (λ(_,x). cexp_ok_bind x ∧ cexp_wf x) l2)
+Proof
+  Induct
+  >- simp [my_function_def] >>
+  PairCases >> simp [my_function_def, PULL_EXISTS] >>
+  rpt $ gen_tac >>
+  pairarg_tac >>
+  rename [‘my_function_bind _ l’, ‘my_function s h = (s', hd')’, ‘v':: _ = _’] >>
+  asm_rewrite_tac [PAIRED_BETA_CONV $
+                    Term ‘(λ(s',hd'). (λ(s'',tl'). (s'',(v, hd')::tl')) (my_function_bind s' l)) (s',hd')’] >>
+  pairarg_tac >>
+  last_x_assum $ drule_then assume_tac >>
+  rename1 ‘my_function_bind s' l = (s'', tl')’ >>
+  asm_rewrite_tac [PAIRED_BETA_CONV $ Term ‘(λ(s'',tl'). (s'',(v, hd')::tl')) (s'', tl')’] >>
+  strip_tac >> strip_tac >>
+  first_assum $ qspec_then ‘h’ mp_tac >>
+  impl_tac >- simp [list_size_def] >>
+  disch_then $ qspec_then ‘s’ mp_tac >>
+  impl_tac >- simp [] >>
+  disch_then $ qspecl_then [‘s'’, ‘hd'’] mp_tac >>
+  impl_tac >- simp [] >> strip_tac >>
+  qpat_x_assum ‘_ ⇒ _’ mp_tac >> impl_tac
+  >- (reverse conj_tac
+      >- (gs [EVERY_CONJ, EVERY_MEM, FORALL_PROD] >>
+          rpt $ strip_tac >> rpt $ first_x_assum $ drule_then assume_tac >>
+          fs [] >> irule SUBSET_TRANS >>
+          first_x_assum $ irule_at $ Pos hd >> simp []) >>
+      gen_tac >> rename1 ‘cexp_size e < list_size _ _’ >>
+      first_x_assum $ qspec_then ‘e’ assume_tac >>
+      strip_tac >> qpat_x_assum ‘_ ⇒ _’ mp_tac >> impl_tac
+      >- simp [list_size_def] >>
+      strip_tac >> gen_tac >> strip_tac >> first_x_assum drule >>
+      rename1 ‘my_function s3 e’ >> Cases_on ‘my_function s3 e’ >> simp []) >>
+  strip_tac >> gs [] >>
+  conj_tac
+  >- (irule SUBSET_TRANS >> first_x_assum $ irule_at $ Pos hd >> simp []) >>
+  qpat_x_assum ‘_::_ = _’ assume_tac >>
+  dxrule_then assume_tac EQ_SYM >>
+  simp [] >> gs [EVERY_CONJ, EVERY_MEM] >>
+  conj_tac
+  >- (conj_tac >> irule SUBSET_TRANS >> metis_tac []) >>
+  qpat_x_assum ‘my_function _ _ = _’ mp_tac >>
+  rpt $ pop_assum kall_tac >>
+  Cases_on ‘h’ >> simp [cexp_ok_bind_def, my_function_def] >>
+  pairarg_tac >> rw [] >> simp [cexp_ok_bind_def]
+QED
+
+
+Theorem my_function_row_lemma:
+  ∀l s l2 s2. my_function_row s l = (s2, l2) ∧
+              (∀e. cexp_size e < list_size (cexp_size o SND o SND) l ⇒
+                   ∀s. vars_ok s ∧ freevars (exp_of e) ⊆ set_of s ∧ cexp_wf e ∧ boundvars (exp_of e) ⊆ set_of s ⇒
+                       ∀s2 e2. (s2, e2) = my_function s e ⇒
+                               cexp_wf e2 ∧
+                               vars_ok s2 ∧ set_of s ⊆ set_of s2 ∧ boundvars (exp_of e2) ⊆ set_of s2 ∧
+                               freevars (exp_of e2) ⊆ set_of s2 ∧
+                               (∀s3. DISJOINT s3 (boundvars (exp_of e2) ∪ freevars (exp_of e2))
+                                     ⇒ exp_rel s3 (exp_of e) (exp_of e2))) ⇒
+              vars_ok s ∧
+              EVERY (λ(v, vs, e). freevars (exp_of (e)) ⊆ set_of s ∧ boundvars (exp_of e) ⊆ set_of s
+                                  ∧ set (MAP explode vs) ⊆ set_of s) l ∧
+              EVERY (λ(v, vs, e). cexp_wf e ∧ ALL_DISTINCT vs) l
+              ⇒ vars_ok s2 ∧ set_of s ⊆ set_of s2 ∧
+                EVERY (λ(v, vs, e). freevars (exp_of (e)) ⊆ set_of s2 ∧ boundvars (exp_of e) ⊆ set_of s2
+                                    ∧ set (MAP explode vs) ⊆ set_of s2) l2 ∧
+                MAP (FST o SND) l = MAP (FST o SND) l2 ∧
+                MAP FST l = MAP FST l2 ∧
+                EVERY (λ(v, vs, e). cexp_wf e ∧ ALL_DISTINCT vs) l2 ∧
+                (∀s3. EVERY (λ(_, vs, e2). DISJOINT s3 (set (MAP explode vs)
+                                                        ∪ boundvars (exp_of e2) ∪ freevars (exp_of e2))) l2
+                      ⇒ LIST_REL (λ(_, _, e) (_, _, e2). exp_rel s3 (exp_of e) (exp_of e2)) l l2)
+Proof
+  Induct
+  >- simp [my_function_def] >>
+  PairCases >> simp [my_function_def, PULL_EXISTS] >>
+  rpt $ gen_tac >> pairarg_tac >>
+  rename [‘my_function_row _ l’, ‘my_function s h = (s', hd')’, ‘(v, vs, _)::_’] >>
+  asm_rewrite_tac [PAIRED_BETA_CONV $
+                    Term ‘(λ(s',hd'). (λ(s'',tl'). (s'',(v, vs, hd')::tl')) (my_function_row s' l)) (s',hd')’] >>
+  pairarg_tac >>
+  last_x_assum $ drule_then assume_tac >>
+  rename1 ‘my_function_row s' l = (s'', tl')’ >>
+  asm_rewrite_tac [PAIRED_BETA_CONV $ Term ‘(λ(s'',tl'). (s'', (v, vs, hd')::tl')) (s'', tl')’] >>
+  strip_tac >> strip_tac >>
+  first_assum $ qspec_then ‘h’ mp_tac >>
+  impl_tac >- simp [list_size_def] >>
+  disch_then $ qspec_then ‘s’ mp_tac >>
+  impl_tac >- simp [] >>
+  disch_then $ qspecl_then [‘s'’, ‘hd'’] mp_tac >>
+  impl_tac >- simp [] >> strip_tac >>
+  qpat_x_assum ‘_ ⇒ _’ mp_tac >> impl_tac
+  >- (reverse conj_tac
+      >- (gs [EVERY_CONJ, EVERY_MEM] >>
+          rpt $ strip_tac >> rpt $ first_x_assum $ drule_then assume_tac >>
+          pairarg_tac >>
+          fs [] >> rpt $ strip_tac >>
+          irule SUBSET_TRANS >>
+          first_x_assum $ irule_at $ Pos hd >> simp []) >>
+      gen_tac >> rename1 ‘cexp_size e < list_size _ _’ >>
+      first_x_assum $ qspec_then ‘e’ assume_tac >>
+      strip_tac >> qpat_x_assum ‘_ ⇒ _’ mp_tac >> impl_tac
+      >- simp [list_size_def] >>
+      strip_tac >> gen_tac >> strip_tac >> first_x_assum drule >>
+      rename1 ‘my_function s3 e’ >> Cases_on ‘my_function s3 e’ >> simp []) >>
+  strip_tac >> gs [] >>
+  conj_tac
+  >- (irule SUBSET_TRANS >> first_x_assum $ irule_at $ Pos hd >> simp []) >>
+  qpat_x_assum ‘_::_ = _’ assume_tac >>
+  dxrule_then assume_tac EQ_SYM >>
+  simp [] >> gs [EVERY_CONJ, EVERY_MEM] >>
+  rpt $ conj_tac >>
+  irule SUBSET_TRANS
+  >- metis_tac []
+  >- metis_tac []
+  >- (irule_at Any SUBSET_TRANS >> metis_tac [])
+QED
+
+Theorem cexp_ok_bind_soundness:
+  ∀e. cexp_wf e ∧ cexp_ok_bind e ⇒ ok_bind (exp_of e)
+Proof
+  Cases >> simp [cexp_ok_bind_def, cexp_wf_def] >>
+  rename1 ‘MAP explode l’ >>
+  Cases_on ‘l’ >> gs []
+QED
+
+Theorem lets_for_boundvars_freevars:
+  ∀l v n x s len. freevars (lets_for len v n (MAPi (λi v. (i, v)) l) x) ⊆ s
+              ∧ boundvars (lets_for len v n (MAPi (λi v. (i, v)) l) x) ⊆ s
+              ⇒ freevars x ⊆ s ∧ boundvars x ⊆ s
+Proof
+  Induct using SNOC_INDUCT
+  \\ simp [lets_for_def, indexedListsTheory.MAPi_APPEND, SNOC_APPEND, lets_for_APPEND]
+  \\ rw []
+  \\ last_x_assum $ dxrule_all_then assume_tac
+  \\ gvs [freevars_def, boundvars_def, SUBSET_DEF]
+  \\ rw [] \\ metis_tac []
+QED
+
+Theorem boundvars_lets_for:
+  ∀l v n x len. boundvars (lets_for len v n (MAPi (λi v. (i, v)) l) x) = boundvars x ∪ (set l)
+Proof
+  Induct using SNOC_INDUCT
+  \\ simp [lets_for_def, indexedListsTheory.MAPi_APPEND, SNOC_APPEND, lets_for_APPEND]
+  \\ rw [boundvars_def, SET_EQ_SUBSET, SUBSET_DEF] \\ gvs []
+QED
+
+Theorem boundvars_Disj:
+  ∀pats w e. boundvars (Disj w pats) ⊆ {w} ∪ boundvars e
+Proof
+  Induct >> simp [FORALL_PROD, Disj_def, boundvars_def]
+QED
+
+Theorem boundvars_rows_of_SOME_lemma:
+  ∀rows w pats e. boundvars e ⊆ boundvars (thunk_exp_of$rows_of w rows (SOME (pats, e)))
+Proof
+  Induct \\ gs [FORALL_PROD, thunk_exp_ofTheory.rows_of_def, boundvars_def, boundvars_Disj]
+  \\ rw []
+  \\ irule SUBSET_TRANS
+  \\ pop_assum $ irule_at Any
+  \\ rename1 ‘rows_of w _ (SOME (pats, _))’
+  \\ qexists_tac ‘w’ \\ qexists_tac ‘pats’ \\ simp []
+QED
+
+Theorem boundvars_rows_of_SOME_NONE:
+  ∀rows w pats e. boundvars (thunk_exp_of$rows_of w rows (SOME (pats, e))) =
+                  boundvars (thunk_exp_of$rows_of w rows NONE) ∪ boundvars e
+Proof
+  Induct \\ gs [FORALL_PROD, thunk_exp_ofTheory.rows_of_def, boundvars_def]
+  >- (gen_tac \\ Induct
+      \\ simp [FORALL_PROD, Disj_def, boundvars_def])
+  \\ simp [UNION_ASSOC]
+QED
+
+Theorem freevars_rows_of_SOME_NONE:
+  ∀rows w pats e. freevars (thunk_exp_of$rows_of w rows (SOME (pats, e))) =
+                  freevars (thunk_exp_of$rows_of w rows NONE) ∪ freevars e ∪ (if pats = [] then {} else {w})
+Proof
+  Induct \\ gs [FORALL_PROD, thunk_exp_ofTheory.rows_of_def, freevars_def]
+  >- (gen_tac \\ Induct
+      \\ simp [FORALL_PROD, Disj_def, freevars_def]
+      \\ simp [GSYM UNION_ASSOC]
+      \\ pop_assum kall_tac
+      \\ gen_tac \\ simp [SET_EQ_SUBSET, SUBSET_DEF] \\ rw [])
+  \\ simp [UNION_ASSOC]
+QED
+
+Theorem exp_rel_lets_for:
+  ∀l n1 n2 x y len s. exp_rel s x y
+                ⇒ exp_rel s (lets_for len n1 n2 l x) (lets_for len n1 n2 l y)
+Proof
+  Induct \\ gvs [lets_for_def, FORALL_PROD]
+  \\ rw [] \\ irule exp_rel_Let
+  \\ irule_at Any exp_rel_Let
+  \\ last_x_assum $ drule_then $ irule_at Any
+  \\ gvs [exp_rel_def]
+QED
+
+Theorem my_function_soundness:
+  ∀s. vars_ok s ∧ freevars (exp_of e) ⊆ set_of s ∧ cexp_wf e ∧ boundvars (exp_of e) ⊆ set_of s ⇒
+      ∀s2 e2. (s2, e2) = my_function s e ⇒
+              cexp_wf e2 ∧
+              vars_ok s2 ∧ set_of s ⊆ set_of s2 ∧ boundvars (exp_of e2) ⊆ set_of s2 ∧
+              freevars (exp_of e2) ⊆ set_of s2 ∧
+              (∀s3. DISJOINT s3 (boundvars (exp_of e2) ∪ freevars (exp_of e2)) ⇒ exp_rel s3 (exp_of e) (exp_of e2))
+Proof
+  completeInduct_on ‘cexp_size e’ >>
+  Cases >> simp [cexp_size_def, my_function_def, boundvars_def, freevars_def, cexp_wf_def]
+  >- simp [exp_rel_Var]
+  >~[‘Prim _ _’]
+  >- (strip_tac >> gen_tac >> strip_tac >>
+      rpt gen_tac >> strip_tac >>
+      pairarg_tac >> gvs [] >>
+      rename [‘my_function_list s l = (s2, l2)’] >>
+      qspecl_then [‘l’, ‘s’, ‘l2’, ‘s2’] mp_tac my_function_list_lemma >>
+      asm_rewrite_tac [] >> impl_tac
+      >- (gen_tac >> strip_tac >>
+          rename1 ‘cexp_size arg < _’ >>
+          last_x_assum $ qspec_then ‘cexp_size arg’ mp_tac >>
+          simp [GSYM size_eq] >>
+          disch_then $ qspec_then ‘arg’ assume_tac >>
+          gs []) >>
+      last_x_assum kall_tac >>
+      gs [BIGUNION_SUBSET, cexp_wf_def, EVERY_CONJ, EVERY_MEM, MEM_MAP,
+          PULL_EXISTS, boundvars_def, freevars_def] >>
+      rw []
+      >- (pop_assum $ qspec_then ‘{}’ assume_tac >> gs [] >>
+          rename1 ‘args_ok c _’ >>
+          Cases_on ‘c’ >> gs [LIST_REL_EL_EQN, args_ok_def] >>
+          rw [] >> gs [my_function_def] >>
+          rpt $ (pairarg_tac >> gvs []))
+      >- (irule exp_rel_Prim >>
+          rename1 ‘exp_rel s3’ >>
+          first_x_assum $ qspec_then ‘s3’ mp_tac >> gs [] >>
+          simp [LIST_REL_EL_EQN, EL_MAP]))
+  >~[‘Apps _ _’]
+  >- (strip_tac >> gen_tac >> strip_tac >>
+      rpt gen_tac >> strip_tac >>
+      pairarg_tac >> gs [] >> pairarg_tac >> gs [] >>
+      rename [‘my_function s e = (s2, e2)’, ‘my_function_list s2 l = (s3, l2)’] >>
+      qspecl_then [‘l’, ‘s2’, ‘l2’, ‘s3’] mp_tac my_function_list_lemma >>
+      asm_rewrite_tac [] >> impl_tac
+      >- (gen_tac >> strip_tac >>
+          rename1 ‘cexp_size arg < _’ >>
+          last_x_assum $ qspec_then ‘cexp_size arg’ mp_tac >>
+          simp [GSYM size_eq] >>
+          disch_then $ qspec_then ‘arg’ assume_tac >>
+          gs []) >>
+      last_x_assum $ qspec_then ‘cexp_size e’ assume_tac >> gs [] >>
+      pop_assum $ qspec_then ‘e’ assume_tac >> gs [] >>
+      pop_assum $ drule_then assume_tac >>
+      gs [boundvars_Apps, freevars_Apps, BIGUNION_SUBSET, cexp_wf_def, EVERY_CONJ] >>
+      impl_tac
+      >- (gs [EVERY_MEM, MEM_MAP, PULL_EXISTS] >> rw [] >>
+          irule SUBSET_TRANS >>
+          last_x_assum $ drule_then $ irule_at $ Pos hd >> simp []) >>
+      rw []
+      >- simp [SF ETA_ss]
+      >- (strip_tac >> gs [])
+      >- gs [SUBSET_DEF]
+      >- gs [SUBSET_DEF]
+      >- gs [MEM_MAP, EVERY_MEM]
+      >- gs [SUBSET_DEF]
+      >- gs [MEM_MAP, EVERY_MEM]
+      >- (irule exp_rel_Apps >>
+          gs [EVERY_MEM, MEM_MAP, PULL_EXISTS] >>
+          first_x_assum $ drule_all_then assume_tac >>
+          gs [LIST_REL_EL_EQN, EL_MAP]))
+  >~[‘Lams _ _’]
+  >- (rename1 ‘cexp_size e’ >> strip_tac >>
+      gs [PULL_FORALL] >>
+      rpt $ gen_tac >> strip_tac >>
+      last_x_assum $ qspec_then ‘e’ assume_tac >> gs [] >>
+      last_x_assum $ drule_then assume_tac >> gs [freevars_Lams, boundvars_Lams, DIFF_SUBSET] >>
+      pairarg_tac >> gs [freevars_Lams, boundvars_Lams] >>
+      strip_tac >> gs [] >>
+      rename1 ‘exp_rel s3 _ _’ >> first_x_assum $ qspec_then ‘s3’ mp_tac >>
+      simp [] >> impl_tac
+      >- (gs [SUBSET_DEF, boundvars_Lams, freevars_Lams, DISJOINT_ALT] >>
+          rw [] >>
+          last_x_assum $ drule_then assume_tac >> gs []) >>
+      rw [exp_rel_Lams, cexp_wf_def]
+      >- gs [SUBSET_DEF]
+      >- gs [SUBSET_DEF]
+      >- (first_x_assum irule >>
+          gs [DISJOINT_ALT] >> rw [] >>
+          first_x_assum $ dxrule_then assume_tac >>
+          rename1 ‘¬MEM x (MAP explode l)’ >>
+          Cases_on ‘MEM x (MAP explode l)’ >> gs []))
+  >~[‘my_function _ (Let opt x y)’]
+  >- (strip_tac >> gs [PULL_FORALL] >>
+      rpt $ gen_tac >> strip_tac >> fs [] >> strip_tac >>
+      rename1 ‘exp_rel s3’ >>
+      rename1 ‘my_function s’ >>
+      Cases_on ‘opt’ >> simp []
+      >- (last_assum $ qspecl_then [‘x’, ‘s’, ‘FST (my_function s x)’, ‘SND (my_function s x)’, ‘s3’] mp_tac >>
+          gs [freevars_def, boundvars_def, my_function_Let_NONE] >>
+          strip_tac >>
+          last_x_assum $ qspecl_then [‘y’, ‘FST (my_function s x)’, ‘FST (my_function (FST (my_function s x)) y)’,
+                                      ‘SND (my_function (FST (my_function s x)) y)’, ‘s3’] mp_tac >>
+          simp [] >> strip_tac >>
+          pairarg_tac >> gs [] >>
+          pairarg_tac >> gvs [SUBSET_DEF, cexp_wf_def, boundvars_def, freevars_def] >>
+          rw [] >> gs [] >>
+          irule exp_rel_Let >> simp []) >>
+      Cases_on ‘dest_Lam x’
+      >- (last_assum $ qspecl_then [‘x’, ‘s’, ‘FST (my_function s x)’, ‘SND (my_function s x)’, ‘s3’] mp_tac >>
+          gs [freevars_def, boundvars_def, my_function_Let_SOME_dLam_is_NONE] >>
+          strip_tac >>
+          last_x_assum $ qspecl_then [‘y’, ‘FST (my_function s x)’, ‘FST (my_function (FST (my_function s x)) y)’,
+                                      ‘SND (my_function (FST (my_function s x)) y)’, ‘s3’] mp_tac >>
+          simp [] >> impl_tac
+          >- (gs [SUBSET_DEF] >>
+              rw [] >> rename1 ‘v ∈ _’ >>
+              rpt $ first_x_assum $ qspec_then ‘v’ assume_tac >> gs [] >>
+              rename1 ‘v ≠ explode x2’ >>
+              Cases_on ‘v = explode x2’ >> gs []) >>
+          simp [] >> strip_tac >>
+          pairarg_tac >> gs [] >>
+          pairarg_tac >> gvs [SUBSET_DEF, cexp_wf_def, boundvars_def, freevars_def] >>
+          rw [] >> gs [] >>
+          irule exp_rel_Let >> simp [] >>
+          first_x_assum irule >>
+          gs [DISJOINT_ALT] >> rw [] >>
+          rename [‘explode v1 ∉ s3’, ‘v2 ∈ freevars _’] >>
+          Cases_on ‘v2 = explode v1’ >> simp []) >>
+      Cases_on ‘x’ >> gs [dest_Lam_def, my_function_def] >>
+      pairarg_tac >> gs [] >>
+      pairarg_tac >> gs [] >>
+      pairarg_tac >> gs [] >>
+      rename1 ‘check_hypothesis (b1 ∧ b2) x' s_vars’ >> Cases_on ‘check_hypothesis (b1 ∧ b2) x' s_vars’
+      >~[‘¬check_hypothesis _ _ _’]
+      >- (rename1 ‘cexp_size (Lam l x2)’ >>
+          last_assum $ qspecl_then [‘Lam l x2’, ‘s’, ‘FST (my_function s (Lam l x2))’,
+                                    ‘SND (my_function s (Lam l x2))’, ‘s3’] assume_tac >>
+          gs [boundvars_def, freevars_def] >>
+          last_x_assum $ qspecl_then [‘y’, ‘FST (my_function s (Lam l x2))’,
+                                      ‘FST (my_function (FST (my_function s (Lam l x2))) y)’,
+                                      ‘SND (my_function (FST (my_function s (Lam l x2))) y)’, ‘s3’] mp_tac >>
+          simp [] >> impl_tac
+          >- (gs [SUBSET_DEF] >> rw [] >> rename1 ‘v ∈ _’ >>
+              rpt $ first_x_assum $ qspec_then ‘v’ assume_tac >> gs [] >>
+              rename1 ‘v ≠ explode x2’ >>
+              Cases_on ‘v = explode x2’ >> gs []) >>
+          strip_tac >> gs [my_function_def, cexp_wf_def, SUBSET_DEF] >>
+          rw [] >> irule_at Any exp_rel_Let >> simp [] >>
+          first_x_assum irule >> simp [] >>
+          gs [DISJOINT_ALT] >> rw [] >>
+          rename [‘explode v1 ∉ s3’, ‘v2 ∈ freevars _’] >>
+          Cases_on ‘v2 = explode v1’ >> simp []) >>
+      gs [] >> pairarg_tac >> gs [] >>
+      rename1 ‘invent_var _ _ = (v2, _)’ >>
+      rename1 ‘cexp_size (Lam l x2)’ >>
+      last_assum $ qspecl_then [‘Lam l x2’, ‘s’, ‘FST (my_function s (Lam l x2))’,
+                                ‘SND (my_function s (Lam l x2))’, ‘{explode v2} ∪ s3’] assume_tac >>
+      gs [boundvars_def, freevars_def] >>
+      last_x_assum $ qspecl_then [‘y’, ‘FST (my_function s (Lam l x2))’,
+                                  ‘FST (my_function (FST (my_function s (Lam l x2))) y)’,
+                                  ‘SND (my_function (FST (my_function s (Lam l x2))) y)’,
+                                  ‘{explode v2} ∪ s3’] mp_tac >>
+      simp [] >> impl_tac
+      >- (gs [SUBSET_DEF] >> rw [] >> rename1 ‘v ∈ _’ >>
+          rpt $ first_x_assum $ qspec_then ‘v’ assume_tac >> gs [] >>
+          rename1 ‘v ≠ explode x2’ >>
+          Cases_on ‘v = explode x2’ >> gs []) >>
+      strip_tac >> gs [my_function_def, cexp_wf_def, boundvars_def, boundvars_Lams, boundvars_Apps,
+                       freevars_Apps, freevars_Lams, freevars_def] >>
+      drule_then assume_tac find_forcing_soundness >>
+      gs [] >>
+      rw []
+      >- (strip_tac >> dxrule_then assume_tac REV_NOT_EMPTY >> fs [] >>
+          dxrule_then assume_tac REV_NOT_EMPTY >> fs [] >>
+          dxrule_then assume_tac REV_merge_inside >> gs [REV_REVERSE_LEM])
+      >- (gs [REV_REVERSE_LEM, GSYM MAP_REVERSE, EVERY_APPEND] >>
+          gs [EVERY_EL, EL_MAP, EL_MAP2, cexp_wf_def] >>
+          rw [cexp_wf_def])
+      >- (strip_tac >> dxrule_then assume_tac REV_NOT_EMPTY >> gs [REV_REVERSE_LEM] >>
+          rename1 ‘MAP2 _ (REVERSE bL) l = []’ >>
+          Cases_on ‘l’ >> fs [] >> qspec_then ‘bL’ assume_tac SNOC_CASES >> gs [])
+      >- (dxrule_then assume_tac invent_var_thm >> gs [])
+      >- (dxrule_then assume_tac invent_var_thm >> gs [SUBSET_DEF])
+      >- (dxrule_then assume_tac invent_var_thm >> gs [REV_REVERSE_LEM, MAP_REVERSE, SUBSET_DEF] >>
+          rw []
+          >- (dxrule_then assume_tac $ iffLR MEM_MAP >> gs [] >>
+              dxrule_then assume_tac thunk_Forcing_LambdasTheory.MEM_MAP_FILTER_ZIP >>
+              gs [MEM_MAP, PULL_EXISTS, MEM_REVERSE])
+          >- (gs [MEM_MAP, PULL_EXISTS] >>
+              dxrule_then assume_tac MEM_merge_inside >>
+              gs [MEM_REVERSE]))
+      >- (dxrule_then assume_tac invent_var_thm >> gs [SUBSET_DEF, SF DNF_ss] >>
+          rw [] >> first_x_assum $ dxrule_then assume_tac >>
+          gs [] >>
+          rename1 ‘REV l []’ >> rename1 ‘x ∈ freevars _’ >>
+          Cases_on ‘MEM x (MAP explode l)’ >> gs [])
+      >- (dxrule_then assume_tac invent_var_thm >> gs [SUBSET_DEF])
+      >- (simp [BIGUNION_SUBSET, REV_REVERSE_LEM, MAP_REVERSE, MEM_MAP, PULL_EXISTS, EXISTS_PROD] >>
+          rw [] >> simp [exp_of_def, boundvars_def] >>
+          pop_assum mp_tac >> gs [REV_REVERSE_LEM] >>
+          simp [MEM_EL, PULL_EXISTS] >>
+          rw [EL_MAP2, boundvars_def])
+      >- (dxrule_then assume_tac invent_var_thm >> gs [SUBSET_DEF])
+      >- (dxrule_then assume_tac invent_var_thm >> gs [SUBSET_DEF])
+      >- (dxrule_then assume_tac invent_var_thm >> gs [SUBSET_DEF])
+      >- (dxrule_then assume_tac invent_var_thm >> gs [SUBSET_DEF, SF DNF_ss] >>
+          rw [] >> first_x_assum $ dxrule_then assume_tac >>
+          gs [] >>
+          rename1 ‘REV l []’ >> rename1 ‘x ∈ freevars _’ >>
+          Cases_on ‘MEM x (MAP explode l)’ >> gs [])
+      >- (simp [DIFF_SUBSET, UNION_SUBSET] >>
+          conj_tac
+          >- (simp [BIGUNION_SUBSET, REV_REVERSE_LEM, MAP_REVERSE, PULL_EXISTS] >>
+              rw []
+              >- (dxrule_then assume_tac $ iffLR MEM_MAP >> fs [] >>
+                  dxrule_then assume_tac $ iffLR MEM_MAP >> fs [] >>
+                  dxrule_then assume_tac $ iffLR MEM_MAP >> fs [] >>
+                  dxrule_then assume_tac thunk_Forcing_LambdasTheory.MEM_MAP_FILTER_ZIP >>
+                  gs [] >> simp [SUBSET_DEF, freevars_def, MEM_MAP]) >>
+              pop_assum mp_tac >> simp [MEM_MAP, PULL_EXISTS, MEM_EL, EL_MAP2] >>
+              rw [] >> simp [exp_of_def, freevars_def, MEM_MAP, EL_MEM])
+          >- (dxrule_then assume_tac invent_var_thm >> gs [SUBSET_DEF]))
+      >- (gs [REV_REVERSE_LEM, MAP2_ZIP, GSYM MAP_REVERSE, GSYM FILTER_REVERSE] >>
+          irule exp_rel_Let_Lams_combine_bis >>
+          gs [exp_rel_Lams, UNION_COMM] >>
+          first_x_assum $ irule_at $ Pos last >>
+          qpat_x_assum ‘_ ∧ _ ⇒ exp_rel _ _ (lets_force _ _)’ mp_tac >>
+          impl_tac
+          >- (rw []
+              >- (dxrule_then assume_tac invent_var_thm >>
+                  strip_tac >> gs [SUBSET_DEF])
+              >- (dxrule_then assume_tac invent_var_thm >>
+                  strip_tac >> gs [SUBSET_DEF])
+              >- (‘∀v : string -> bool s1 s2. DISJOINT s2 v ∧ s1 = s2 ⇒ DISJOINT s1 v’ by simp [] >>
+                  pop_assum irule >>
+                  irule_at (Pos hd) FEQUAL >>
+                  irule_at (Pos hd) FEQUAL2 >> irule_at (Pos hd) FEQUAL >>
+                  irule_at Any REVERSE_ZIP >>
+                  conj_asm1_tac
+                  >- (simp [] >>
+                      irule EQ_LENGTH_FILTER_ZIP >>
+                      simp [LENGTH_merge_inside]) >>
+                  simp [boundvars_lets_force] >>
+                  gs [DISJOINT_ALT] >> rw [] >>
+                  dxrule_then assume_tac $ iffLR MEM_MAP >> fs [] >>
+                  dxrule_then assume_tac thunk_Forcing_LambdasTheory.MEM_MAP_FILTER_ZIP >>
+                  ‘∀l y. MEM y l ⇒ MEM (explode y) (MAP explode l)’ by simp [MEM_MAP] >>
+                  pop_assum $ dxrule_then assume_tac >> gs [MAP_REVERSE])
+              >- (rename1 ‘MEM (explode v2) (MAP explode l)’ >>
+                  Cases_on ‘MEM (explode v2) (MAP explode l)’ >> simp [] >>
+                  dxrule_then assume_tac invent_var_thm >>
+                  strip_tac >> gs [SUBSET_DEF])
+              >- (gs [DISJOINT_ALT] >> rpt $ strip_tac >>
+                  rename1 ‘x ∉ _ ∨ MEM x (MAP explode l)’ >>
+                  Cases_on ‘MEM x (MAP explode l)’ >> simp [] >> strip_tac >>
+                  dxrule_then assume_tac in_freevars_lets_force >>
+                  gs [MAP_REVERSE]
+                  >- (first_x_assum $ dxrule_then assume_tac >> gs []) >>
+                  dxrule MEM_MAP_ZIP >> impl_tac
+                  >- (simp [] >> irule EQ_LENGTH_FILTER_ZIP >>
+                      simp [LENGTH_merge_inside]) >>
+                  strip_tac >> dxrule_then assume_tac $ iffLR MEM_MAP >>
+                  gs [] >> dxrule_then assume_tac thunk_Forcing_LambdasTheory.MEM_MAP_FILTER_ZIP >>
+                  gs [MEM_MAP])) >>
+          strip_tac >>
+          dxrule_then assume_tac exp_rel_lets_force_left >> gs [] >>
+          first_assum $ irule_at $ Pos last >>
+          rename1 ‘ZIP (bL, merge_inside (REVERSE l) bL l3)’ >>
+          ‘LENGTH bL = LENGTH (merge_inside (REVERSE l) bL l3)’ by gs [LENGTH_merge_inside] >>
+          rename1 ‘REVERSE (ZIP (bL2, REVERSE l))’ >>
+          ‘LENGTH bL2 = LENGTH l’ by gs [LIST_REL_EL_EQN] >>
+          gs [REVERSE_ZIP, MAP_FILTER_ZIP, MAP_REVERSE] >>
+          qspecl_then [‘bL’, ‘REVERSE l’, ‘l3’, ‘explode’] mp_tac MAP_merge_inside >>
+          impl_tac >- simp [GSYM REVERSE_ZIP, FILTER_REVERSE] >>
+          strip_tac >> gs [] >>
+          qspecl_then [‘MAP explode (REVERSE l)’, ‘bL’, ‘MAP explode l3’] mp_tac REVERSE_merge_inside >>
+          impl_tac
+          >- (simp [] >> irule EQ_TRANS >>
+              rename1 ‘ZIP (bL, MAP explode (REVERSE l))’ >>
+              qspecl_then [‘FILTER FST $ ZIP (bL, MAP explode (REVERSE l))’, ‘SND’] (irule_at Any) LENGTH_MAP >>
+              irule_at Any EQ_TRANS >> irule_at (Pos last) FEQUAL >>
+              irule_at Any MAP_FILTER_ZIP >>
+              simp []) >>
+          strip_tac >> gs [MAP_REVERSE] >>
+          dxrule_then assume_tac check_hypothesis_soundness >>
+          qexists_tac ‘REVERSE (MAP explode l3)’ >>
+          qexists_tac ‘MAP explode l’ >>
+          qexists_tac ‘REVERSE bL2’ >> qexists_tac ‘REVERSE bL’ >>
+          rw []
+          >- gs [DISJOINT_SYM]
+          >- (dxrule_then assume_tac invent_var_thm >> strip_tac >> gs [SUBSET_DEF])
+          >- (gs [DISJOINT_ALT] >> rpt $ strip_tac >>
+              rename1 ‘x ∈ freevars (exp_of _)’ >>
+              rpt $ first_x_assum $ qspec_then ‘x’ assume_tac >> gs [])
+          >- (dxrule_then assume_tac invent_var_thm >> strip_tac >> gs [SUBSET_DEF])
+          >- gs [MEM_MAP]
+          >- gs [MEM_MAP]
+          >- (dxrule_then assume_tac invent_var_thm >> strip_tac >> gs [SUBSET_DEF])
+          >- (dxrule_then assume_tac invent_var_thm >> strip_tac >> gs [MEM_MAP, SUBSET_DEF])
+          >- gs [ALL_DISTINCT_APPEND, MEM_MAP, PULL_EXISTS]
+          >- (dxrule_then assume_tac invent_var_thm >> strip_tac >> gs [boundvars_to_lets_force, SUBSET_DEF])
+          >- (dxrule_then assume_tac invent_var_thm >> strip_tac >> gs [SUBSET_DEF])
+          >- (dxrule_then assume_tac invent_var_thm >> strip_tac >> gs [SUBSET_DEF])
+          >- (dxrule_then assume_tac invent_var_thm >> strip_tac >> gs [SUBSET_DEF] >>
+              rename1 ‘_ ∈ freevars  _ ∧ _ ≠ explode x' ⇒ _ ∈ _’ >>
+              Cases_on ‘explode v2 = explode x'’ >> gs [])
+          >- (AP_THM_TAC >> AP_TERM_TAC >>
+              AP_THM_TAC >> AP_TERM_TAC >>
+              irule EQ_TRANS >> irule_at (Pos hd) REVERSE_ZIP >>
+              simp [] >> irule_at Any EQ_LENGTH_FILTER_ZIP >>
+              conj_asm1_tac
+              >- (irule LENGTH_merge_inside >> simp [] >>
+                  irule_at Any EQ_LENGTH_FILTER_ZIP >> simp []) >>
+              simp [] >> AP_TERM_TAC >> simp [] >>
+              conj_tac
+              >- (‘LENGTH l = LENGTH bL’ by simp [] >> pop_assum mp_tac >>
+                  qpat_x_assum ‘LENGTH l3 = LENGTH (FILTER FST (ZIP (bL, REVERSE l)))’ mp_tac >>
+                  rpt $ pop_assum kall_tac >>
+                  qid_spec_tac ‘l3’ >> qid_spec_tac ‘bL’ >>
+                  Induct_on ‘l’ using SNOC_INDUCT >> simp [merge_inside_def, REVERSE_SNOC] >>
+                  gen_tac >> Cases >> simp [] >>
+                  IF_CASES_TAC >> simp [merge_inside_def] >>
+                  Cases >> simp [merge_inside_def]) >>
+              simp [GSYM MAP_REVERSE, GSYM FILTER_REVERSE, REVERSE_ZIP])
+          >- (AP_THM_TAC >> AP_TERM_TAC >> AP_TERM_TAC >> MK_COMB_TAC
+              >- (AP_TERM_TAC >> simp [MAP_FILTER_ZIP] >>
+                  AP_TERM_TAC >> AP_TERM_TAC >> AP_TERM_TAC >> simp [] >>
+                  gs [MAP_MAP_o, combinTheory.o_DEF])
+              >- (irule LIST_EQ >> simp [EL_MAP2, EL_MAP, EL_ZIP] >>
+                  rw [exp_of_def]))
+          >- (irule EQ_TRANS >> irule_at Any LENGTH_REVERSE >>
+              once_rewrite_tac [GSYM FILTER_REVERSE] >>
+              simp [REVERSE_ZIP, EQ_LENGTH_FILTER_ZIP])
+          >- (rpt $ qpat_x_assum ‘LIST_REL _ _ _’ mp_tac >>
+              dxrule exp_rel_freevars >>
+              rpt $ pop_assum kall_tac >>
+              rw [] >> gs [LIST_REL_EVERY_ZIP, GSYM REVERSE_ZIP] >>
+              irule $ iffLR EVERY_REVERSE >>
+              ‘LENGTH (REVERSE (ZIP (bL, bL2))) = LENGTH (MAP explode l)’ by simp [] >>
+              dxrule_then assume_tac REVERSE_ZIP >>
+              asm_rewrite_tac [REVERSE_REVERSE])))
+  >~[‘Letrec _ _’]
+  >- (strip_tac >> gen_tac >> strip_tac >>
+      rpt gen_tac >> strip_tac >>
+      pairarg_tac >> gs [] >> pairarg_tac >> gs [] >>
+      rename [‘my_function s e = (s2, e2)’, ‘my_function_bind s2 l = (s3, l2)’] >>
+      qspecl_then [‘l’, ‘s2’, ‘l2’, ‘s3’] mp_tac my_function_bind_lemma >>
+      asm_rewrite_tac [] >> impl_tac
+      >- (gen_tac >> strip_tac >>
+          rename1 ‘cexp_size arg < _’ >>
+          last_x_assum $ qspec_then ‘cexp_size arg’ mp_tac >>
+          simp [size_eq2] >>
+          disch_then $ qspec_then ‘arg’ assume_tac >>
+          gs []) >>
+      last_x_assum $ qspec_then ‘cexp_size e’ assume_tac >> gs [] >>
+      pop_assum $ qspec_then ‘e’ assume_tac >> gs [] >>
+      pop_assum $ drule_then assume_tac >>
+      gs [boundvars_def, freevars_def, BIGUNION_SUBSET, cexp_wf_def, EVERY_CONJ] >>
+      ‘freevars (exp_of e) ⊆ set_of s’
+        by (gs [SUBSET_DEF, SF DNF_ss, MEM_MAP, PULL_EXISTS, FORALL_PROD] >>
+            gen_tac >> rename1 ‘x ∈ freevars _’ >>
+            Cases_on ‘MEM (implode x) (MAP FST l)’
+            >- (gs [MEM_MAP, FST_THM] >> pairarg_tac >>
+                gvs [] >>
+                first_x_assum $ dxrule_then assume_tac >>
+                gs [explode_implode]) >>
+            strip_tac >> last_x_assum irule >>
+            gs [MEM_MAP]) >>
+      impl_tac
+      >- (gs [EVERY_MEM, SUBSET_DEF, MEM_MAP] >>
+          gs [FORALL_PROD, EXISTS_PROD, PULL_EXISTS] >>
+          rw []
+          >- (rename1 ‘x ∈ set_of _’ >>
+              Cases_on ‘MEM (implode x) (MAP FST l)’
+              >- (gs [MEM_MAP, FST_THM] >> pairarg_tac >>
+                  gvs [] >>
+                  first_x_assum $ dxrule_then assume_tac >>
+                  gs [explode_implode]) >>
+              last_x_assum irule >> last_x_assum irule >>
+              gs [MEM_MAP] >> metis_tac [])
+          >- (last_x_assum $ drule_then assume_tac >> fs [])
+          >- (last_x_assum $ drule_then assume_tac >>
+              last_x_assum $ drule_then assume_tac >> gs [])) >>
+      strip_tac >>
+      rw []
+      >- (strip_tac >> gs [])
+      >- gs []
+      >- gs [SUBSET_DEF]
+      >- gs [SUBSET_DEF]
+      >- (gs [MEM_MAP, EVERY_MEM] >>
+          pairarg_tac >> gs [] >> pairarg_tac >> gvs [] >>
+          first_x_assum $ drule_then assume_tac >>
+          first_x_assum $ dxrule_then assume_tac >> gs [])
+      >- (rename1 ‘MAP FST l = MAP FST l2’ >>
+          ‘MAP FST (MAP (λ(n,x'). (explode n,exp_of x')) l) = MAP FST (MAP (λ(n,x'). (explode n,exp_of x')) l2)’
+            suffices_by gs [SUBSET_DEF] >>
+          irule LIST_EQ >>
+          qpat_x_assum ‘MAP _ _ = MAP _ _’ mp_tac >>
+          once_rewrite_tac [GSYM LIST_REL_eq] >>
+          strip_tac >> dxrule_then assume_tac $ iffLR LIST_REL_EL_EQN >>
+          gs [EL_MAP] >> rw [] >>
+          pairarg_tac >> gs [] >> pairarg_tac >> gs [] >>
+          first_x_assum $ drule_then assume_tac >> gs [])
+      >- (gs [SUBSET_DEF] >> rw []
+          >- gs [] >>
+          dxrule_then assume_tac $ iffLR MEM_MAP >> gs [] >>
+          dxrule_then assume_tac $ iffLR MEM_MAP >> gs [EVERY_MEM] >>
+          first_x_assum $ drule_then kall_tac >>
+          first_x_assum $ dxrule_then assume_tac >>
+          pairarg_tac >> gs [])
+      >- (irule exp_rel_Letrec >>
+          conj_tac
+          >- (irule LIST_EQ >>
+              qpat_x_assum ‘MAP _ _ = MAP _ _’ mp_tac >>
+              once_rewrite_tac [GSYM LIST_REL_eq] >>
+              strip_tac >> dxrule_then assume_tac $ iffLR LIST_REL_EL_EQN >>
+              gs [EL_MAP] >> rw [] >>
+              pairarg_tac >> gs [] >> pairarg_tac >> gs [] >>
+              first_x_assum $ drule_then assume_tac >> gs []) >>
+          gs [MAP_MAP_o, combinTheory.o_DEF, LAMBDA_PROD, EVERY_CONJ] >>
+          ‘DISJOINT (freevars (exp_of e2) ∪ BIGUNION (set (MAP (λ(p1, p2). freevars (exp_of p2)) l2))) s3'’
+            by (gs [DISJOINT_ALT] >>
+                rw [] >> rename1 ‘x ∉ s3'’ >>
+                Cases_on ‘MEM x (MAP (λ(p1, p2). explode p1) l2)’ >> gs [] >>
+                first_x_assum irule >> gs [] >>
+                metis_tac []) >>
+          qpat_x_assum ‘DISJOINT (_ ∪ _ DIFF _) _’ kall_tac >>
+          gs [] >>
+          qpat_x_assum ‘∀s3. EVERY _ _ ⇒ LIST_REL _ _ _’ $ qspec_then ‘s3'’ mp_tac >>
+          impl_tac
+          >- (gs [EVERY_MEM, MEM_MAP, PULL_EXISTS, FORALL_PROD] >>
+              rw [] >> first_x_assum $ drule_then irule) >>
+          strip_tac >>
+          gs [EVERY_EL, LIST_REL_EL_EQN, EL_MAP] >>
+          rw []
+          >- (last_x_assum $ drule_then assume_tac >> pairarg_tac >> gs [] >>
+              drule_all_then irule cexp_ok_bind_soundness)
+          >- (last_x_assum $ drule_then assume_tac >>
+              first_x_assum $ drule_then assume_tac >>
+              pairarg_tac >> gs [] >>
+              pairarg_tac >> gs [] >>
+              drule_all_then assume_tac cexp_ok_bind_soundness >>
+              rename1 ‘exp_rel _ e_in e_out’ >>
+              Cases_on ‘e_in’ >> gs [ok_bind_def, exp_rel_def])
+          >- (first_x_assum $ drule_then assume_tac >>
+              pairarg_tac >> gs [] >>
+              pairarg_tac >> gs [])))
+  >~[‘rows_of _ _ _’]
+
+  >- (strip_tac >> gen_tac >> strip_tac >>
+      rpt gen_tac >> strip_tac >>
+      pairarg_tac >> gs [] >> pairarg_tac >> gs [] >>
+      rename [‘my_function_row s row = (s2, row2)’] >>
+      qspecl_then [‘row’, ‘s’, ‘row2’, ‘s2’] mp_tac my_function_row_lemma >>
+      asm_rewrite_tac [] >> impl_tac
+      >- (gen_tac >> strip_tac >>
+          rename1 ‘cexp_size arg < _’ >>
+          last_x_assum $ qspec_then ‘cexp_size arg’ mp_tac >>
+          simp [size_eq_case, list_size_MAP] >>
+          disch_then $ qspec_then ‘arg’ assume_tac >>
+          gs []) >>
+      impl_tac
+      >- (reverse conj_tac
+          >- (gs [EVERY_MEM, FORALL_PROD, SF DNF_ss] >>
+              rw [] >> first_x_assum irule >>
+              first_x_assum $ irule_at Any) >>
+          qpat_x_assum ‘freevars _ ⊆ _’ mp_tac >>
+          qpat_x_assum ‘boundvars _ ⊆ _’ mp_tac >>
+          rpt $ pop_assum kall_tac >> Induct_on ‘row ’ >>
+          simp [FORALL_PROD, rows_of_def, boundvars_def, freevars_def] >>
+          rpt gen_tac >> strip_tac >> strip_tac >>
+          drule_all_then assume_tac lets_for_boundvars_freevars >>
+          simp [] >>
+          qpat_x_assum ‘boundvars (lets_for _ _ _ _ _) ⊆ _’ mp_tac >>
+          simp [boundvars_lets_for]) >>
+      strip_tac >>
+      conj_tac
+      >- (rw [cexp_wf_def]
+          >- (qpat_x_assum ‘EVERY _ row2’ mp_tac >>
+              rpt $ pop_assum kall_tac >>
+              simp [EVERY_MEM, FORALL_PROD, SF DNF_ss] >>
+              rw [] >>
+              first_x_assum $ drule_then irule)
+          >- (strip_tac >> gs [])
+          >- gs []
+          >- (rename1 ‘OPTION_ALL _ eopt1’ >>
+              Cases_on ‘eopt1’ >> gs [] >>
+              pairarg_tac >> gs [] >>
+              pairarg_tac >> gvs [])
+          >- (qpat_x_assum ‘_ = (_, _)’ mp_tac >>
+              CASE_TAC >> simp [] >>
+              CASE_TAC >> pairarg_tac >> simp [] >>
+              rw [] >> gs [cexp_size_def] >>
+              rename1 ‘my_function s2 e1 = (s3, e2)’ >>
+              last_x_assum $ qspec_then ‘cexp_size e1’ mp_tac >> simp [] >>
+              disch_then $ qspec_then ‘e1’ mp_tac >> simp [] >>
+              disch_then $ qspec_then ‘s2’ mp_tac >> simp [] >>
+              impl_tac
+              >- (gs [freevars_rows_of] >>
+                  assume_tac boundvars_rows_of_SOME_lemma >>
+                  gs [SUBSET_DEF]) >>
+              simp [])) >>
+      rename1 ‘OPTION_ALL _ eopt1’ >>
+      conj_asm1_tac
+      >- (Cases_on ‘eopt1’ >> gs [] >> pairarg_tac >> gs [] >>
+          pairarg_tac >> gvs [] >>
+          rename1 ‘my_function s2 e = (s3, e2)’ >>
+          last_x_assum $ qspec_then ‘cexp_size e’ mp_tac >> simp [cexp_size_def] >>
+          disch_then $ qspec_then ‘e’ mp_tac >> simp [] >>
+          disch_then $ qspec_then ‘s2’ mp_tac >> simp [] >>
+          impl_tac
+          >- (gs [freevars_rows_of] >>
+              assume_tac boundvars_rows_of_SOME_lemma >>
+              gs [SUBSET_DEF]) >>
+          simp []) >>
+      conj_asm1_tac
+      >- (Cases_on ‘eopt1’ >> gs [] >> pairarg_tac >> gs [] >>
+          pairarg_tac >> gvs [] >>
+          rename1 ‘my_function s2 e = (s3, e2)’ >>
+          last_x_assum $ qspec_then ‘cexp_size e’ mp_tac >> simp [cexp_size_def] >>
+          disch_then $ qspec_then ‘e’ mp_tac >> simp [] >>
+          disch_then $ qspec_then ‘s2’ mp_tac >> simp [] >>
+          impl_tac
+          >- (gs [freevars_rows_of] >>
+              assume_tac boundvars_rows_of_SOME_lemma >>
+              gs [SUBSET_DEF]) >>
+          gs [SUBSET_DEF]) >>
+      rename1 ‘boundvars (rows_of (explode m) (MAP _ row2) (OPTION_MAP _ eopt')) ⊆ set_of s3’ >>
+      ‘set_of s2 ⊆ set_of s3’
+        by (Cases_on ‘eopt1’ >> gs [] >>
+            pairarg_tac >> gs [] >>
+            pairarg_tac >> gs [] >>
+            rename1 ‘my_function s2 e = (s3, e')’ >>
+            last_x_assum $ qspec_then ‘cexp_size e’ mp_tac >> simp [cexp_size_def] >>
+            disch_then $ qspec_then ‘e’ mp_tac >> simp [] >>
+            disch_then $ qspec_then ‘s2’ mp_tac >> simp [] >>
+            impl_tac
+            >- (gs [freevars_rows_of] >>
+                assume_tac boundvars_rows_of_SOME_lemma >>
+                gs [SUBSET_DEF]) >>
+            simp []) >>
+      conj_asm1_tac
+      >- (‘boundvars (rows_of (explode m) (MAP (λ(c,vs,x). (explode c,MAP explode vs,exp_of x)) row2) NONE)
+           ⊆ set_of s3’
+            by (qpat_x_assum ‘EVERY _ row2’ kall_tac >>
+                qpat_x_assum ‘EVERY _ row2’ mp_tac >>
+                qpat_x_assum ‘set_of s2 ⊆ set_of s3’ mp_tac >>
+                rpt $ pop_assum kall_tac >> Induct_on ‘row2’ >>
+                simp [rows_of_def, boundvars_def, FORALL_PROD, boundvars_lets_for] >>
+                rw [] >> gs [SUBSET_DEF]) >>
+          Cases_on ‘eopt1’ >> gs [] >>
+          pairarg_tac >> gs [] >>
+          pairarg_tac >> gvs [boundvars_rows_of_SOME_NONE] >>
+          rename1 ‘my_function s2 e = (s3, e2)’ >>
+          last_x_assum $ qspec_then ‘cexp_size e’ mp_tac >> simp [cexp_size_def] >>
+          disch_then $ qspec_then ‘e’ mp_tac >> simp [] >>
+          disch_then $ qspec_then ‘s2’ mp_tac >> simp [] >>
+          impl_tac
+          >- (gs [freevars_rows_of] >>
+              assume_tac boundvars_rows_of_SOME_lemma >>
+              gs [SUBSET_DEF]) >>
+          simp []) >>
+      conj_asm1_tac
+      >- (‘freevars (rows_of (explode m) (MAP (λ(c,vs,x). (explode c,MAP explode vs,exp_of x)) row2) NONE)
+           ⊆ set_of s3’
+            by (qpat_x_assum ‘EVERY _ row2’ kall_tac >>
+                qpat_x_assum ‘EVERY _ row2’ mp_tac >>
+                ‘explode m ∈ set_of s3’
+                  by (Cases_on ‘row’ >> gs [] >>
+                      rename1 ‘my_function_row _ (h::_)’ >> PairCases_on ‘h’ >>
+                      gs [rows_of_def, freevars_def] >>
+                      gs [SUBSET_DEF]) >>
+                pop_assum mp_tac >>
+                dxrule_then (drule_then mp_tac) SUBSET_TRANS >>
+                qpat_x_assum ‘set_of s2 ⊆ set_of s3’ mp_tac >>
+                rpt $ pop_assum kall_tac >> Induct_on ‘row2’ >>
+                simp [rows_of_def, freevars_def, FORALL_PROD] >>
+                rw [SUBSET_DEF] >>
+                assume_tac freevars_lets_for >>
+                gs [SET_EQ_SUBSET, SUBSET_DEF, SF DNF_ss] >>
+                rename1 ‘x ∈ freevars _’ >>
+                Cases_on ‘x = explode m’ >> gs [] >>
+                last_x_assum $ drule_then assume_tac >>
+                gs []) >>
+          Cases_on ‘eopt1’ >> gs [] >>
+          pairarg_tac >> gs [] >>
+          pairarg_tac >> gvs [freevars_rows_of_SOME_NONE] >>
+          reverse conj_tac
+          >- (qpat_x_assum ‘explode m ∈ _’ mp_tac >>
+              rpt $ qpat_x_assum ‘set_of _ ⊆ set_of _’ mp_tac >>
+              rpt $ pop_assum kall_tac >> rw [] >>
+              gs [SUBSET_DEF]) >>
+          rename1 ‘my_function s2 e = (s3, e2)’ >>
+          last_x_assum $ qspec_then ‘cexp_size e’ mp_tac >> simp [cexp_size_def] >>
+          disch_then $ qspec_then ‘e’ mp_tac >> simp [] >>
+          disch_then $ qspec_then ‘s2’ mp_tac >> simp [] >>
+          impl_tac
+          >- (gs [freevars_rows_of] >>
+              assume_tac boundvars_rows_of_SOME_lemma >>
+              gs [SUBSET_DEF]) >>
+          simp [])
+
+      >- (rw [] >> rename1 ‘exp_rel s4 _ _’ >>
+          first_x_assum $ qspec_then ‘s4’ mp_tac >>
+          impl_tac
+          >- (pop_assum mp_tac >>
+              pop_assum mp_tac >>
+              rpt $ pop_assum kall_tac >>
+              Induct_on ‘row2’ >>
+              simp [FORALL_PROD, rows_of_def, freevars_def, boundvars_def] >>
+              rw [] >> gs [boundvars_lets_for] >>
+              assume_tac freevars_lets_for >>
+              gs [SET_EQ_SUBSET, SUBSET_DEF, SF DNF_ss, DISJOINT_ALT] >>
+              rw [] >> rename [‘x ∈ freevars _’, ‘LENGTH p_1'’] >>
+              Cases_on ‘MEM x (MAP explode p_1')’ >> gs [] >>
+              Cases_on ‘x = explode m’ >> gs []) >>
+          Cases_on ‘eopt1’ >> gs []
+          >- (qpat_x_assum ‘MAP (FST o SND) _ = MAP (FST o SND) _’ mp_tac >>
+              qpat_x_assum ‘MAP FST _ = MAP FST _’ mp_tac >>
+              rpt $ pop_assum kall_tac >>
+              qid_spec_tac ‘row2’ >>
+              Induct_on ‘row’ >> gs [PULL_EXISTS, FORALL_PROD, PULL_FORALL, rows_of_def]
+              >- simp [exp_rel_def] >>
+              rw [] >>
+              irule exp_rel_If >>
+              conj_tac >- simp [exp_rel_def] >>
+              conj_tac
+              >- simp [exp_rel_lets_for]
+              >- (last_x_assum irule >> gs [])) >>
+          pairarg_tac >> gs [] >>
+          pairarg_tac >> gs [] >>
+          rename1 ‘my_function s2 e = (s3, e2)’ >>
+          last_x_assum $ qspec_then ‘cexp_size e’ mp_tac >> simp [cexp_size_def] >>
+          disch_then $ qspec_then ‘e’ mp_tac >> simp [] >>
+          disch_then $ qspec_then ‘s2’ mp_tac >> simp [] >>
+          impl_tac
+          >- (gs [freevars_rows_of] >>
+              assume_tac boundvars_rows_of_SOME_lemma >>
+              gs [SUBSET_DEF]) >>
+          strip_tac >>
+          first_x_assum $ qspec_then ‘s4’ mp_tac >>
+          gvs [freevars_rows_of_SOME_NONE, boundvars_rows_of_SOME_NONE] >>
+          qpat_x_assum ‘MAP (FST o SND) _ = MAP (FST o SND) _’ mp_tac >>
+          qpat_x_assum ‘MAP FST _ = MAP FST _’ mp_tac >>
+          rpt $ pop_assum kall_tac >>
+          qid_spec_tac ‘row2’ >>
+          Induct_on ‘row’ >> gs [PULL_EXISTS, FORALL_PROD, PULL_FORALL, rows_of_def]
+          >- (simp [exp_rel_def] >> disch_then kall_tac >>
+              rename1 ‘Disj _ l’ >>
+              Induct_on ‘l’ >> simp [FORALL_PROD, Disj_def, exp_rel_def]) >>
+          simp [exp_rel_def, exp_rel_lets_for]))
+  >~[‘Delay (exp_of e)’]
+  >- (strip_tac >> gs [PULL_FORALL] >>
+      last_x_assum $ qspec_then ‘e’ assume_tac >>
+      gen_tac >> pairarg_tac >> gs [boundvars_def, freevars_def, exp_rel_def] >>
+      gen_tac >> strip_tac >> simp [cexp_wf_def] >>
+      last_x_assum $ dxrule_then assume_tac >> gs [])
+  >~[‘Box (exp_of e)’]
+  >- (strip_tac >> gs [PULL_FORALL] >>
+      last_x_assum $ qspec_then ‘e’ assume_tac >>
+      gen_tac >> pairarg_tac >> gs [boundvars_def, freevars_def, exp_rel_def] >>
+      gen_tac >> strip_tac >> simp [cexp_wf_def] >>
+      last_x_assum $ dxrule_then assume_tac >> gs [])
+  >~[‘Force (exp_of e)’]
+  >- (strip_tac >> gs [PULL_FORALL] >>
+      last_x_assum $ qspec_then ‘e’ assume_tac >>
+      gen_tac >> pairarg_tac >> gs [boundvars_def, freevars_def, exp_rel_def] >>
+      gen_tac >> strip_tac >> simp [cexp_wf_def] >>
+      last_x_assum $ dxrule_then assume_tac >> gs [])
+QED
+
+val _ = export_theory ();
